pulse/examples/dsls/mini_steel/Pulse.Checker.Pure.fsti
@@ -13,15 +13,14 @@ module RTB = FStar.Tactics.Builtins
 val check_universe (f0:RT.fstar_top_env) (g:env) (t:term)
   : T.Tac (u:universe & universe_of f0 g t u)
   
-      
-val check_tot_univ (allow_inst:bool) (f:RT.fstar_top_env) (g:env) (t:term)
+val check_tot_univ (f:RT.fstar_top_env) (g:env) (t:term)
   : T.Tac (t:term  &
            u:universe &
            ty:term &
            universe_of f g ty u &
            typing f g t ty)
 
-val check_tot (allow_inst:bool) (f:RT.fstar_top_env) (g:env) (t:term)
+val check_tot (f:RT.fstar_top_env) (g:env) (t:term)
   : T.Tac (t:term &
            ty:term &
            typing f g t ty)
@@ -29,19 +28,19 @@ val check_tot (allow_inst:bool) (f:RT.fstar_top_env) (g:env) (t:term)
 val check_tot_with_expected_typ (f:RT.fstar_top_env) (g:env) (e:term) (t:term)
   : T.Tac (e:term & typing f g e t)
 
-val check_tot_no_inst (f:RT.fstar_top_env) (g:env) (t:term)
+val check_with_core (f:RT.fstar_top_env) (g:env) (t:term)
   : T.Tac (ty:term &
            typing f g t ty)
-
-val check_vprop_no_inst (f:RT.fstar_top_env)
-                        (g:env)
-                        (t:term)
-  : T.Tac (tot_typing f g t Tm_VProp)
 
 val check_vprop (f:RT.fstar_top_env)
                 (g:env)
                 (t:term)
   : T.Tac (t:term & _:tot_typing f g t Tm_VProp)
+
+val check_vprop_with_core (f:RT.fstar_top_env)
+                          (g:env)
+                          (t:term)
+  : T.Tac (tot_typing f g t Tm_VProp)
 
 val get_non_informative_witness (f:RT.fstar_top_env) (g:env) (u:universe) (t:term)
   : T.Tac (non_informative_t f g u t)
